\include{"../preamble.tex"}
\title{ECE 131A HW 3}
\begin{document}
\maketitle
\section*{Problem 1}
Then this must be a geometric distribution, so the pmf would be 
$$p(Y=y)=(1-p)^{y-1}p$$
\section*{Problem 2}
\subsection*{(a)}
$$\boxed{\frac{\frac{1}{1}}{\sum_{n=1}^{10}\frac{1}{n^s}}}$$
\subsection*{(b)}
$$\boxed{\frac{\sum_{n=6}^{10}\frac{1}{n^s}}{\sum_{n=1}^{10}\frac{1}{n^s}}}$$
\section*{Problem 3}
\subsection*{(a)}
we have
$$k\int_{0}^{1}x^2(1-x)^2dx=1$$
$$k\int_{0}^{1}x^2-2x^3+x^4dx=1$$
$$k\left[\frac{x^3}{3}-\frac{2x^4}{4}+\frac{x^5}{5}\right]_{0}^{1}=1$$
$$k\left(\frac{1}{3}-\frac{2}{4}+\frac{1}{5}\right)=1$$
$$\boxed{k=30}$$
\subsection*{(b)}
\begin{align*}
    P(X\geq \frac{3}{4})&=30\int_{\frac{3}{4}}^{1}x^2(1-x)^2dx\\
    &=30\left[\frac{x^3}{3}-\frac{2x^4}{4}+\frac{x^5}{5}\right]_{\frac{3}{4}}^{1}\\
    &=\boxed{0.103515625}
\end{align*}
\section*{Problem 4}
\subsection*{(a)}
Let the price of gas be a random variable $X$, then we have that the
total cost $Y=12X+1$, thus
$$E[Y]=E[12X+1]=12E[X]+1=12\cdot4.40+1=\boxed{53.8}$$
\subsection*{(b)}
We have
$$\text{Var}(X)=12^2\text{Var}(Y)=12^2\left(\frac{1}{12}(0.2)^2\right)=0.48$$
\section*{Problem 5}
\subsection*{(a)}
We have that as a function of the distance $d$ of the shorter part in porportion
to the entire rod,
so evenly distributed from $0$ to $0.5$. then the ratio of the lengths is
$$r(d)=\frac{d}{1-d}$$ 
Since this function is invertible for the range of $d\in[0,0.5]$, we have
$$d(r)=\frac{r}{r+1}$$
thus we have that the probability density function is
$$f_R(r)=f_d(d(r))\left|\frac{d d(r)}{dr}\right|$$
$$f_R(r)=\boxed{\frac{2}{(r+1)^2}}$$
\subsection*{(b)}
$$E[R]=\int_{0}^{1}\frac{2r}{(r+1)^2}dr=0.38629436112$$
\subsection*{(c)}
$$E[R^2]=\int_{0}^{1}\frac{2r^2}{(r+1)^2}dr=0.22741127776$$
$$Var(R)=E[R^2]-E[R]^2=\boxed{0.07818794432}$$
\section*{Problem 6}
This is an erlang distibution, with $k=7$, this's cdf 
$P(X\leq 10)=1-\sum_{n=0}^{6}\frac{(10\lambda)^n}{n!}e^{-10\lambda}$, so we have
that the probability of wait for more than 10 minutes is
$$1-P(X\leq 10)=\boxed{\sum_{n=0}^{6}\frac{(10\lambda)^n}{n!}e^{-10\lambda}}$$
\section*{Problem 7}
\subsection*{(a)}
Since the probability fo getting $X=1$ is $0$ for a countinuous random variable,
we have that 
$$P(Y\geq1)=P(X\geq0)=\boxed{1}$$
\subsection*{(b)}
$$P(Y\geq10)=P(X\geq9)=\boxed{e^{-27}}$$
\subsection*{(c)}
$$P(Y\geq x)=P(X\geq x-1)=\boxed{e^{-3(x-1)}}$$
\section*{Problem 8}
The standard z score for a standard normal $Z$ to have 
$P(Z\leq z)=0.1492$ is $-1.03987$, so we have that
$$x=\mu+\sigma z=-1.03987\cdot2\sqrt{2}+22=\boxed{19.0588034858}$$
\section*{Problem 9}
\subsection*{(a)}
Let $X=\int_{-\infty}^{\infty}e^{-x^2}dx$, then we have that
\begin{align*}
    X^2&=\int_{-\infty}^{\infty}e^{-x^2}dx\int_{-\infty}^{\infty}e^{-y^2}dydx\\
    &=\int_{-\infty}^{\infty}\int_{-\infty}^{\infty}e^{-x^2-y^2}dxdy\\
    &=\int_{0}^{2\pi}\int_{0}^{\infty}e^{-r^2}rdrd\theta\\
    &=2\pi\int_{0}^{\infty}e^{-r^2}rdr\\
    &=\pi
\end{align*}
Thus we have that $X=\sqrt{\pi}$, then we have that 
\begin{align}
    \int_{-\infty}^{\infty}f(x)dx&=\frac{1}{\sigma\sqrt{2\pi}}\int_{-\infty}^{\infty}e^{-\frac{(x-\mu)^2}{2\sigma^2}}dx
\end{align}
Let $y=x-\mu$, then we have that
\begin{align*}
    \int_{-\infty}^{\infty}f(x)dx&=\frac{1}{\sigma\sqrt{2\pi}}\int_{-\infty}^{\infty}e^{-\frac{y^2}{2\sigma^2}}dy
\end{align*}
Let $z=\frac{y}{\sigma\sqrt{2}}$, then we have that $dz=\frac{dy}{\sigma\sqrt{2}}$,
thus we have that 
\begin{align*}
    \int_{-\infty}^{\infty}f(x)dx&=\frac{1}{\sqrt{\pi}}\int_{-\infty}^{\infty}e^{-z^2}dz\\
    &=1
\end{align*}
Thus $f(x)$ could be a density function
\subsection*{(b)}
we have through integration by parts
\begin{align*}
    \sqrt{2\pi}(1-\Phi(x))&=\int_{x}^{+\infty}e^{-\frac{y^2}{2}}dy\\
    &=\left.-y^{-1}e^{-\frac{y^2}{2}}\right|_{x}^{\infty}-\int_{x}^{\infty}y^{-2}e^{-\frac{y^2}{2}}dy\\
    &=x^{-1}e^{-\frac{x^2}{2}}-\int_{x}^{\infty}y^{-2}e^{-\frac{y^2}{2}}dy\\
    &= x^{-1}e^{-\frac{x^2}{2}}+\left.y^{-3}e^{-\frac{y^2}{2}}\right|_{x}^{\infty}+\int_{x}^{\infty}y^{-3}e^{-\frac{y^2}{2}}dy\\
    &=(x^{-1}-x^{-3})e^{-\frac{x^2}{2}}+\int_{x}^{\infty}y^{-3}e^{-\frac{y^2}{2}}dy
\end{align*}
Therefore since $\int_{x}^{\infty}y^{-3}e^{-\frac{y^2}{2}}dy>0$ and $\int_{x}^{\infty}y^{-2}e^{-\frac{y^2}{2}}dy> 0$ we have
$$(x^{-1}-x^{-3})e^{-\frac{x^2}{2}}<\sqrt{2\pi}(1-\Phi(x))<x^{-1}e^{-\frac{x^2}{2}}$$
\subsection*{(c)}
For $x>0$ we have that 
$$P(X>x+\frac{a}{x}|X>x)=\frac{P(X>x+\frac{a}{x})}{P(X>x)}$$
Now we use the squeeze theorem, we have that 
$$\frac{\left(x+\frac{a}{x}\right)^{-1}e^{-\frac{1}{2}(x+\frac{a}{x})^2}}
{(x^{-1}-x^{-3})e^{-\frac{x^2}{2}}}
>\frac{P(X>x+\frac{a}{x})}{P(X>x)}>
\frac{\left(\left(x+\frac{a}{x}\right)^{-1}-
\left(x+\frac{a}{x}\right)^{-3}\right)e^{-\frac{1}{2}(x+\frac{a}{x})^2}}
    {x^{-1}e^{-\frac{x^2}{2}}}$$
since $x+\frac{a}{x}\to x$ as $x\to\infty$ we have that 
$$\lim_{x\to\infty}\frac{\left(x+\frac{a}{x}\right)^{-1}e^{-\frac{1}{2}(x+\frac{a}{x})^2}}
{(x^{-1}-x^{-3})e^{-\frac{x^2}{2}}}=e^{-a}$$
and
$$\lim_{x\to\infty}\frac{\left(\left(x+\frac{a}{x}\right)^{-1}-
\left(x+\frac{a}{x}\right)^{-3}\right)e^{-\frac{1}{2}(x+\frac{a}{x})^2}}
    {x^{-1}e^{-\frac{x^2}{2}}}=e^{-a}$$
Thus we have that 
$$P\left(X>x+\frac{a}{x}|X>x\right)\to e^{-a}$$
As $x\to\infty$ 
\end{document}
