\include{"../preamble.tex"}
\title{ECE 131A HW 6}
\begin{document}
\maketitle
\section*{Problem 1}
We have that assuming the number of pens is large, 
then the total lifetime of the pens is distributed according to
a normal with mean $n$ and variance $n$ therefore we have that we want
to find a $n$ such that 
$$-2.32635=\frac{15-n}{\sqrt{n}}$$
solving this we get that $n=27.11$ therefore the student would need
$\boxed{28}$ pens in order for the probability of having a pen 
to run out during a semester to be greater than $0.99$
\section*{Problem 2}
The number of errors in 100 transmission can be estimated
as a normal distribution with mean of 15 and variance of $100\cdot0.15\cdot0.85=12.75$,
therefore the probability of having more than 20 errors has a corresponding 
$Z$ value of $1.4$ and therefore a corresponding probability of
$\boxed{0.91924}$.
\section*{Problem 3}
\subsection*{(a)}
We have that 
$$\Sigma^{-1}=\begin{bmatrix}
\frac{3}{5}&\frac{1}{5}\\ \frac{1}{5}&\frac{2}{5}\end{bmatrix}$$
And 
$$det(\Sigma)=5$$
Therefore we have that 
$$\Sigma^{-1}(\mu-X)=\frac{1}{5}\begin{bmatrix}
    3(\mu_1-x_1)+(\mu_2-x_2)\\
    (\mu_1-x_1)+2(\mu_2-x_2)
\end{bmatrix}$$
and therefore we have that
$$(\mu-X)^T\Sigma^{-1}(\mu-X)=\frac{3}{5}(\mu_1-x_1)^2+\frac{2}{5}(\mu_2-x_2)(\mu_1-x_1)+\frac{2}{5}(\mu_2-x_2)^2$$
Therefore we have that
$$f(x_1,x_2)=(2\pi)^{-1}\frac{1}{\sqrt{5}}e^{-\frac{3}{10}(1-x_1)^2-\frac{1}{5}(2-x_2)(1-x_1)-\frac{1}{5}(2-x_2)^2}$$
\subsection*{(b)}
We have that Y is distributed as an normal distribution with 
mean $A\mu+B=4$ and variance $A\Sigma A^T=3$ therefore we have that
the pdf of $Y$ is 
$$f(y)=\frac{1}{\sqrt{2\pi3}}e^{-\frac{(y-4)^2}{6}}$$
\subsection*{(c)}
Therefore we have that given that $Z$ is a standard normal distribution
$$P(Y\geq 2)=P(Z\geq \frac{2-4}{\sqrt{3}})=1-0.12425=\boxed{0.87575}$$
\section*{Problem 4}
\subsection*{(a)}
Therefore we have that the covariance matrix is 
$$\Sigma=\begin{bmatrix}
2&1&0\\
1&2&1\\
0&1&2
\end{bmatrix}$$
\subsection*{(b)}
We have that the pdf of $Y$ is
$$f(y_1,y_2,y_3)=(2\pi)^{-\frac{3}{2}}\frac{1}{2}e^{\frac{1}{4}(y_1y_2+y_2y_3)
-\frac{3}{8}(y_1^2+y_2^2+y_3^2)}$$
\subsection*{(c)}
We have that the distirbution for $Y_1$ and $Y_2$ is a 
given by a linear transformation of $[Y_1,Y_2,Y_3]$ with 
$A=\begin{bmatrix}1&0&0\\0&1&0\end{bmatrix}$. Therefore we have 
that this mu is $A\mu=\begin{bmatrix}0\\0\end{bmatrix}$ and
the covariance matrix is $A\Sigma A^T=\begin{bmatrix}2&1\\1&2\end{bmatrix}$.
Therefore we have that 
$$f(y_1,y_2)=\frac{1}{2\pi}\frac{1}{\sqrt{3}}e^{-\frac{1}{3}(y_1^2+y_2^2-y_1y_2)}$$
Likewise we have that the distribution for $Y_1$ and $Y_3$ is a
given by a linear transformation of $[Y_1,Y_2,Y_3]$ with
$A=\begin{bmatrix}1&0&0\\0&0&1\end{bmatrix}$. Therefore we have
that this mu is $A\mu=\begin{bmatrix}0\\0\end{bmatrix}$ and
the covariance matrix is $A\Sigma A^T=\begin{bmatrix}2&0\\0&2\end{bmatrix}$.
Therefore we have that
$$f(y_1,y_3)=\frac{1}{2\pi}\frac{1}{2}e^{-\frac{1}{4}(y_1^2+y_3^2)}$$
\subsection*{(d)}
we can simply use a linear transformation $$A=\begin{bmatrix}1&-1&0\\0&1&-1\\-1 & 0 & 1\end{bmatrix}$$
\section*{Problem 6}
We can approximate the sum of the 64 numbers as a gaussian with 
mean 0 and variance $64\frac{1}{12}=\frac{16}{3}$ therefore we have that
the probability of the sum being greater than 4 is the same as the probability
that a $Z$, a standard normal distribution, is greater than $\frac{4}{\sqrt{\frac{16}{3}}}=\sqrt{3}$, 
which is $1-0.95837=\boxed{0.04163}$.
\section*{Problem 7}
\subsection*{(a)}
We have that 
$$f(y|0)=\frac{1}{2\alpha}e^{-\frac{|y+1|}{\alpha}}$$
\subsection*{(b)}
We have that
$$f(y|1)=\frac{1}{2\alpha}e^{-\frac{|y-1|}{\alpha}}$$
\subsection*{(c)}
We have that
$$f(y)=0.5\frac{1}{2\alpha}e^{-\frac{|y-1|}{\alpha}}+0.5\frac{1}{2\alpha}e^{-\frac{|y+1|}{\alpha}}$$
\subsection*{(d)}
We have that the probability of error given that 
"0" was sent is
$$\int_{0}^{\infty}\frac{1}{2\alpha}e^{-\frac{y+1}{\alpha}}dy=\frac{e^{-\frac{1}{\alpha}}}{2}$$
and the probability of error given that "1" was sent is
$$\int_{-\infty}^{0}\frac{1}{2\alpha}e^{-\frac{1-y}{\alpha}}dy=\frac{e^{-\frac{1}{\alpha}}}{2}$$
\subsection*{(e)}
Therefore we have that the probability of error is
$$\frac{1}{2}\frac{e^{-\frac{1}{\alpha}}}{2}+\frac{1}{2}\frac{e^{-\frac{1}{\alpha}}}{2}=\frac{e^{-\frac{1}{\alpha}}}{2}$$
\section*{Problem 8}
\subsection*{(a)}
$$f_Y(y|X=+1)=\frac{1}{\sqrt{2\pi\sigma^2}}e^{-\frac{(y-1)^2}{2\sigma^2}}$$
$$f_Y(y|X=-1)=\frac{1}{\sqrt{2\pi\sigma^2}}e^{-\frac{(y+1)^2}{2\sigma^2}}$$
\subsection*{(b)}
We have that for $y<0$, $f_Y(y|X=+1)<f_Y(y|X=-1)$ and for $y>0$, $f_Y(y|X=+1)>f_Y(y|X=-1)$
and at $y=0$ we have that $f_Y(y|X=+1)=f_Y(y|X=-1)$. Therefore we have this 
is equivalent to saying that when $Y<0$ we decide "0" and 
when $Y\geq0$ we decide "1".
\subsection*{(c)}
The probability of error given that "0" was sent is
$$\int_{0}^{\infty}\frac{1}{\sqrt{2\pi\sigma^2}}e^{-\frac{(y-1)^2}{2\sigma^2}}dy=0.00003$$
and the probability of error given that "1" was sent is
$$\int_{-\infty}^{0}\frac{1}{\sqrt{2\pi\sigma^2}}e^{-\frac{(y+1)^2}{2\sigma^2}}dy=0.00003$$
\subsection*{(d)}
Therefore we have that the probability of error is
$$\frac{1}{2}\frac{1}{\sqrt{2\pi\sigma^2}}e^{-\frac{(y-1)^2}{2\sigma^2}}+\frac{1}{2}\frac{1}{\sqrt{2\pi\sigma^2}}e^{-\frac{(y+1)^2}{2\sigma^2}}=0.00003$$
\section*{Problem 9}
\subsection*{(a)}
$$\phi_z(t)=\frac{2}{2-it}\cdot \frac{10}{10-it}$$
\subsection{(b)}
$$\phi_z(t)=-\frac{20}{8}\frac{1}{10-it}+\frac{20}{8}\frac{1}{2-it}$$
Computing the inverse fourier transform we get
$$f(z)=\frac{20}{8}e^{-2z}-\frac{20}{8}e^{-10z} \text{ when } z\geq 0 and f(z)=0 \text{ when } z<0$$
\section*{Problem 10}
$$E[T]=\frac{1}{3}\cdot 3+\frac{2}{3}E[T]+\frac{1}{3}(5+7)$$
$$E[T]=15$$
\section*{Problem 11}
\subsection*{(a)}





\end{document}

